## Elektromagnetische Induktion

$B=\mu_{0}\mu_{r} \frac{NI}{l}$
$U_{i}=-N\frac{\mathrm{d}\phi}{\mathrm{d}t}$
$\phi =B\cdot A$

$\begin{split}U_{i}&=-N\frac{\mathrm{d}\phi}{\mathrm{d}t}=-N\frac{\mathrm{d}(B\cdot A)}{\mathrm{d}t}=-N\frac{\mathrm{d}(\cdot\mu_{0}\mu_{r} \frac{NI}{l} A)}{\mathrm{d}t}\\ &=-N\cdot\mu_{0}\mu_{r} \frac{N}{l} A\frac{\mathrm{d}I}{\mathrm{d}t}=-\cdot\mu_{0}\mu_{r} \frac{N^{2} A}{l}\frac{\mathrm{d}I}{\mathrm{d}t}\end{split}$
$U=-L \frac{\mathrm{d}I}{\mathrm{d}t}$
$L=\mu_{0}\mu_{r} \frac{N^{2}A}{l}$